src/program_proof/session/gossip.v
@@ -5,18 +5,18 @@ Section heap.
 
   Context `{hG: !heapGS Σ}.
 
-  Lemma wp_receiveGossip (sv:tuple_of[u64,u64,Slice.t,Slice.t,Slice.t,Slice.t,Slice.t,Slice.t]) (s: Server.t)
-    (msgv:tuple_of[u64,u64,u64,u64,u64,Slice.t,u64,u64,Slice.t,u64,u64,u64,u64,u64,u64,Slice.t,u64,u64]) (msg: Message.t)
+  Lemma wp_receiveGossip (sv: tuple_of[u64,u64,Slice.t,Slice.t,Slice.t,Slice.t,Slice.t,Slice.t]) (s: Server.t)
+    (msgv: tuple_of[u64,u64,u64,u64,u64,Slice.t,u64,u64,Slice.t,u64,u64,u64,u64,u64,u64,Slice.t,u64,u64]) (msg: Message.t)
     (n: nat) c2s s2c len_mo len_ga :
     {{{
-        is_server sv s n n n len_mo n len_ga ∗ 
+        is_server sv s n n n len_mo n len_ga true ∗ 
         is_message msgv msg n c2s s2c ∗
         ⌜is_sorted s .(Server.PendingOperations) /\ is_sorted s .(Server.OperationsPerformed)⌝
     }}}
       receiveGossip (server_val sv) (message_val msgv)
     {{{
         r, RET server_val r;
-        is_server r (coq_receiveGossip s msg) n n n len_mo n len_ga ∗
+        is_server r (coq_receiveGossip s msg) n n n len_mo n len_ga true ∗
         is_message msgv msg n c2s s2c ∗
         ⌜is_sorted (coq_receiveGossip s msg) .(Server.PendingOperations) /\ is_sorted (coq_receiveGossip s msg) .(Server.OperationsPerformed)⌝
     }}}.
@@ -230,17 +230,17 @@ Section heap.
       }
   Qed.
 
-  Lemma wp_acknowledgeGossip (sv:tuple_of[u64,u64,Slice.t,Slice.t,Slice.t,Slice.t,Slice.t,Slice.t]) (s: Server.t)
-    (msgv:tuple_of[u64,u64,u64,u64,u64,Slice.t,u64,u64,Slice.t,u64,u64,u64,u64,u64,u64,Slice.t,u64,u64]) (msg: Message.t)
-    (n: nat) c2s s2c len_vc len_op len_mo len_po len_ga :
+  Lemma wp_acknowledgeGossip (sv: tuple_of[u64,u64,Slice.t,Slice.t,Slice.t,Slice.t,Slice.t,Slice.t]) (s: Server.t)
+    (msgv: tuple_of[u64,u64,u64,u64,u64,Slice.t,u64,u64,Slice.t,u64,u64,u64,u64,u64,u64,Slice.t,u64,u64]) (msg: Message.t)
+    (n: nat) c2s s2c len_vc len_op len_mo len_po len_ga OWN_UnsatisfiedRequests :
     {{{
-        is_server sv s n len_vc len_op len_mo len_po len_ga ∗ 
+        is_server sv s n len_vc len_op len_mo len_po len_ga OWN_UnsatisfiedRequests ∗ 
         is_message msgv msg n c2s s2c
     }}}
       acknowledgeGossip (server_val sv) (message_val msgv)
     {{{
         r, RET r;
-        is_server sv (coq_acknowledgeGossip s msg) n len_vc len_op len_mo len_po len_ga ∗
+        is_server sv (coq_acknowledgeGossip s msg) n len_vc len_op len_mo len_po len_ga OWN_UnsatisfiedRequests ∗
         is_message msgv msg n c2s s2c
     }}}.
   Proof.
@@ -281,16 +281,16 @@ Section heap.
       + iPureIntro. done.
   Qed.
 
-  Lemma wp_getGossipOperations (sv:tuple_of[u64,u64,Slice.t,Slice.t,Slice.t,Slice.t,Slice.t,Slice.t]) (s: Server.t)
-    (serverId: w64) (n: nat) len_vc len_op len_mo len_po len_ga :
+  Lemma wp_getGossipOperations (sv: tuple_of[u64,u64,Slice.t,Slice.t,Slice.t,Slice.t,Slice.t,Slice.t]) (s: Server.t)
+    (serverId: w64) (n: nat) len_vc len_op len_mo len_po len_ga OWN_UnsatisfiedRequests :
     {{{
-        is_server sv s n len_vc len_op len_mo len_po len_ga
+        is_server sv s n len_vc len_op len_mo len_po len_ga OWN_UnsatisfiedRequests
     }}}
       getGossipOperations (server_val sv) #serverId
     {{{
         ns , RET slice_val (ns);
         operation_slice ns (coq_getGossipOperations s serverId) len_mo ∗
-        is_server sv s n len_vc len_op len_mo len_po len_ga
+        is_server sv s n len_vc len_op len_mo len_po len_ga OWN_UnsatisfiedRequests
     }}}.
   Proof.
     TypeVector.des sv.
