src/program_proof/session/processRequest.v
@@ -5,9 +5,9 @@ Section heap.
 
   Context `{hG: !heapGS Σ}.
 
-  Lemma wp_processClientRequest sv s msgv msg (n: nat) (m: nat) len_po len_ga len_s2c :
+  Lemma wp_processClientRequest {OWN_UnsatisfiedRequests: bool} sv s msgv msg (n: nat) (m: nat) len_po len_ga len_s2c :
     {{{
-        is_server sv s n m m m len_po len_ga ∗
+        is_server sv s n m m m len_po len_ga OWN_UnsatisfiedRequests ∗
         is_message msgv msg n m len_s2c ∗
         ⌜SERVER_INVARIANT s⌝
     }}}
@@ -15,7 +15,7 @@ Section heap.
     {{{
         (b: bool) ns nm, RET (#b, server_val ns, message_val nm);
         ⌜b = (coq_processClientRequest s msg).1.1⌝ ∗
-        is_server ns (coq_processClientRequest s msg).1.2 n m m m len_po len_ga ∗
+        is_server ns (coq_processClientRequest s msg).1.2 n m m m len_po len_ga OWN_UnsatisfiedRequests ∗
         is_message nm (coq_processClientRequest s msg).2 n 0%nat (if b then m else 0%nat) ∗
         is_message msgv msg n m len_s2c ∗
         ⌜SERVER_INVARIANT (coq_processClientRequest s msg).1.2⌝
@@ -150,14 +150,14 @@ Section heap.
 
   Lemma wp_processRequest sv s msgv msg (n: nat) len_ga len_s2c :
     {{{
-        is_server sv s n n n n n len_ga ∗
+        is_server sv s n n n n n len_ga true ∗
         is_message msgv msg n n len_s2c ∗
         ⌜SERVER_INVARIANT s⌝
     }}}
       processRequest (server_val sv) (message_val msgv)
     {{{
         ns nms, RET (server_val ns, slice_val nms);
-        is_server ns (coq_processRequest s msg).1 n n n n n len_ga ∗
+        is_server ns (coq_processRequest s msg).1 n n n n n len_ga true ∗
         message_slice nms (coq_processRequest s msg).2 n ∗
         ⌜SERVER_INVARIANT (coq_processRequest s msg).1⌝
     }}}.
@@ -174,7 +174,7 @@ Section heap.
     { wp_apply wp_ref_to. { repeat econstructor; eauto. } iIntros "%succeeded H_succeeded".
       wp_pures. wp_apply wp_ref_to. { repeat econstructor; eauto. } iIntros "%reply H_reply".
       wp_pures. wp_load. replace (processClientRequest (#s .(Server.Id), (#s .(Server.NumberOfServers), (t4, (t3, (t2, (t1, (t0, (t, #()))))))))%V (#msg .(Message.MessageType), (#msg .(Message.C2S_Client_Id), (#msg .(Message.C2S_Server_Id), (#msg .(Message.C2S_Client_OperationType), (#msg .(Message.C2S_Client_Data), (t7, (#msg .(Message.S2S_Gossip_Sending_ServerId), (#msg .(Message.S2S_Gossip_Receiving_ServerId), (t6, (#msg .(Message.S2S_Gossip_Index), (#msg .(Message.S2S_Acknowledge_Gossip_Sending_ServerId), (#msg .(Message.S2S_Acknowledge_Gossip_Receiving_ServerId), (#msg .(Message.S2S_Acknowledge_Gossip_Index), (#msg .(Message.S2C_Client_OperationType), (#msg .(Message.S2C_Client_Data), (t5, (#msg .(Message.S2C_Server_Id), (#msg .(Message.S2C_Client_Number), #()))))))))))))))))))%V) with (processClientRequest (server_val (s .(Server.Id), s .(Server.NumberOfServers), t4, t3, t2, t1, t0, t)) (message_val (msg .(Message.MessageType), msg .(Message.C2S_Client_Id), msg .(Message.C2S_Server_Id), msg .(Message.C2S_Client_OperationType), msg .(Message.C2S_Client_Data), t7, msg .(Message.S2S_Gossip_Sending_ServerId), msg .(Message.S2S_Gossip_Receiving_ServerId), t6, msg .(Message.S2S_Gossip_Index), msg .(Message.S2S_Acknowledge_Gossip_Sending_ServerId), msg .(Message.S2S_Acknowledge_Gossip_Receiving_ServerId), msg .(Message.S2S_Acknowledge_Gossip_Index), msg .(Message.S2C_Client_OperationType), msg .(Message.S2C_Client_Data), t5, msg .(Message.S2C_Server_Id), msg .(Message.S2C_Client_Number)))) by f_equal.
-      wp_apply (wp_processClientRequest with "[H3 H4 H6 H7 H8 H9 H16 H20 H27]"). { iFrame. simplNotation; subst. done. } iIntros "%b %ns %nm (-> & H_server' & H_message' & H_message & %H1_postcondition)".
+      wp_apply (wp_processClientRequest (OWN_UnsatisfiedRequests := true) with "[H3 H4 H6 H7 H8 H9 H16 H20 H27]"). { iFrame. simplNotation; subst. done. } iIntros "%b %ns %nm (-> & H_server' & H_message' & H_message & %H1_postcondition)".
       wp_store. wp_store. wp_pures; lazymatch goal with [ |- envs_entails _ (wp ?s ?E (App ?k ?e)%E ?Q) ] => eapply (tac_wp_store_ty _ _ _ _ _ _ [AppRCtx k]%list); [repeat econstructor; eauto | tc_solve | let l := reply in iAssumptionCore | reflexivity | simpl] end.
       wp_pures. wp_load. wp_if_destruct.
       - wp_load. wp_load. replace message_val with (message_into_val .(to_val)) by reflexivity. wp_apply (wp_SliceAppend with "[$H_s1]"). iIntros "%s2 H_s2".
@@ -194,7 +194,69 @@ Section heap.
       wp_store. wp_load. wp_load. TypeVector.des r. replace (#(W64 2), (zero_val uint64T, (zero_val uint64T, (zero_val uint64T, (zero_val uint64T, (zero_val (slice.T uint64T), (zero_val uint64T, (zero_val uint64T, (zero_val (slice.T (slice.T uint64T * (uint64T * unitT)%ht)), (zero_val uint64T, (#r, (#msg .(Message.S2S_Gossip_Sending_ServerId), (#msg .(Message.S2S_Gossip_Index), (zero_val uint64T, (zero_val uint64T, (zero_val (slice.T uint64T), (zero_val uint64T, (zero_val uint64T, #()))))))))))))))))))%V with (message_into_val .(to_val) (W64 2, W64 0, W64 0, W64 0, W64 0, Slice.nil, W64 0, W64 0, Slice.nil, W64 0, r, msg .(Message.S2S_Gossip_Sending_ServerId), msg .(Message.S2S_Gossip_Index), W64 0, W64 0, Slice.nil, W64 0, W64 0)) by reflexivity.
       wp_apply (wp_SliceAppend with "[$H_s1]"). iIntros "%s2 H_s2". wp_store. wp_pures. wp_apply (wp_ref_to); auto. iIntros "%i H_i". wp_apply (wp_ref_to). { repeat econstructor; eauto. } iIntros "%reply H_reply". wp_pures. wp_apply (wp_ref_to); auto. iIntros "%succeeded H_succeeded". wp_pures. simpl in *.
       rename r into Id, w into NumberOfServers, t13 into UnsatisfiedRequests, t12 into VectorClock, t11 into OperationsPerformed, t10 into MyOperations, t9 into PendingOperations, t8 into GossipAcknowledgements.
-      
+      set (focus := (coq_receiveGossip s msg).(Server.UnsatisfiedRequests)).
+      set (loop_init := (0%nat, (s, [Message.mk 0 0 0 0 0 [] 0 0 [] 0 (s.(Server.Id)) (msg.(Message.S2S_Gossip_Sending_ServerId)) (msg.(Message.S2S_Gossip_Index)) 0 0 [] 0 0]))).
+      set (loop_step := λ acc : nat * (Server.t * list Message.t), λ element : Message.t,
+        let '(i, (s, outGoingRequests)) := acc in
+        let '(succeeded, s, reply) := coq_processClientRequest s element in
+        if succeeded then
+          let UnsatisfiedRequests := coq_deleteAtIndexMessage s.(Server.UnsatisfiedRequests) i in
+          (i, (Server.mk s.(Server.Id) s.(Server.NumberOfServers) UnsatisfiedRequests s.(Server.VectorClock) s.(Server.OperationsPerformed) s.(Server.MyOperations) s.(Server.PendingOperations) s.(Server.GossipAcknowledgements), outGoingRequests ++ [reply]))
+        else
+          ((i + 1)%nat, (s, outGoingRequests))
+      ).
+      set (n := length s .(Server.VectorClock)). rename s into s0. iDestruct "Hr" as "(%H1 & %H2 & H3 & H4 & %H5 & H6 & H7 & H8 & H9 & %H10)"; simplNotation; simpl in *.
+      wp_apply (wp_forBreak_cond
+        ( λ continue, ∃ prevs : list Message.t, ∃ nexts : list Message.t, ∃ s : Server.t, ∃ msgs : list Message.t, ∃ out_going_requests : Slice.t, ∃ index : nat, ∃ msgv : tuple_of [u64,u64,u64,u64,u64,Slice.t,u64,u64,Slice.t,u64,u64,u64,u64,u64,u64,Slice.t,u64,u64], ∃ b : bool, ∃ Id : w64, ∃ NumberOfServers : w64, ∃ UnsatisfiedRequests : Slice.t, ∃ VectorClock : Slice.t, ∃ OperationsPerformed : Slice.t, ∃ MyOperations : Slice.t, ∃ PendingOperations : Slice.t, ∃ GossipAcknowledgements : Slice.t,
+          ⌜focus = prevs ++ nexts⌝ ∗
+          ⌜(index, (s, msgs)) = fold_left loop_step prevs loop_init⌝ ∗
+          outGoingRequests ↦[(slice.T (uint64T * (uint64T * (uint64T * (uint64T * (uint64T * (slice.T uint64T * (uint64T * (uint64T * (slice.T (slice.T uint64T * (uint64T * unitT)) * (uint64T * (uint64T * (uint64T * (uint64T * (uint64T * (uint64T * (slice.T uint64T * (uint64T * (uint64T * unitT)))))))))))))))))))%ht] slice_val out_going_requests ∗
+          i ↦[uint64T] #index ∗
+          reply ↦[(uint64T * (uint64T * (uint64T * (uint64T * (uint64T * (slice.T uint64T * (uint64T * (uint64T * (slice.T (slice.T uint64T * (uint64T * unitT)) * (uint64T * (uint64T * (uint64T * (uint64T * (uint64T * (uint64T * (slice.T uint64T * (uint64T * (uint64T * unitT))))))))))))))))))%ht] message_val msgv ∗
+          succeeded ↦[boolT] #b ∗
+          server ↦[(uint64T * (uint64T * (slice.T (uint64T * (uint64T * (uint64T * (uint64T * (uint64T * (slice.T uint64T * (uint64T * (uint64T * (slice.T (slice.T uint64T * (uint64T * unitT)) * (uint64T * (uint64T * (uint64T * (uint64T * (uint64T * (uint64T * (slice.T uint64T * (uint64T * (uint64T * unitT)))))))))))))))))) * (slice.T uint64T * (slice.T (slice.T uint64T * (uint64T * unitT)) * (slice.T (slice.T uint64T * (uint64T * unitT)) * (slice.T (slice.T uint64T * (uint64T * unitT)) * (slice.T uint64T * unitT))))))))%ht] server_val (Id, NumberOfServers, UnsatisfiedRequests, VectorClock, OperationsPerformed, MyOperations, PendingOperations, GossipAcknowledgements)%core ∗
+          message_slice UnsatisfiedRequests s.(Server.UnsatisfiedRequests) n ∗
+          own_slice_small VectorClock uint64T (DfracOwn 1) s.(Server.VectorClock) ∗
+          operation_slice OperationsPerformed s.(Server.OperationsPerformed) n ∗
+          operation_slice MyOperations s.(Server.MyOperations) n ∗
+          operation_slice PendingOperations s.(Server.PendingOperations) n ∗
+          own_slice_small GossipAcknowledgements uint64T (DfracOwn 1) s.(Server.GossipAcknowledgements) ∗
+          message_slice out_going_requests msgs n ∗
+          ⌜SERVER_INVARIANT s⌝ ∗
+          ⌜length s.(Server.UnsatisfiedRequests) = (index + length nexts)%nat⌝ ∗
+          ⌜drop index s.(Server.UnsatisfiedRequests) = nexts⌝ ∗
+          ⌜length s.(Server.VectorClock) = length s0.(Server.VectorClock)⌝ ∗
+          ⌜(index <= uint.nat UnsatisfiedRequests.(Slice.sz))%nat⌝ ∗
+          ⌜length s.(Server.UnsatisfiedRequests) = uint.nat UnsatisfiedRequests.(Slice.sz)⌝ ∗
+          ⌜continue = false -> nexts = []⌝
+        )%I
+      with "[] [H_outGoingRequests H_server H3 H4 H6 H7 H8 H9 H_message H_s2 H_i H_reply H_succeeded]").
+      { subst Id NumberOfServers. clear Φ UnsatisfiedRequests VectorClock OperationsPerformed MyOperations PendingOperations GossipAcknowledgements.
+        iIntros "%Φ". iModIntro. iIntros "(%prevs & %nexts & %s & %msgs & %out_going_requests & %index & %msgv & %b & %Id & %NumberOfServers & %UnsatisfiedRequests & %VectorClock & %OperationPerformed & %MyOperations & %PendingOperations & %GossipAcknowledgements & %FOCUS & %LOOP & H_outGoingRequests & H_i & H_reply & H_succeeded & H_server & H_UnsatisfiedRequests & H_VectorClock & H_OperationsPerformed & H_MyOperations & H_PendingOperations & H_GossipAcknowledgements & H_out_going_requests & %H_server_invariant & %claim1 & %claim2 & %claim3 & %claim4 & %H_continue) HΦ". iDestruct "H_UnsatisfiedRequests" as "(%msgv1 & [H1_UnsatisfiedRequests H2_UnsatisfiedRequests] & H3_UnsatisfiedRequests)".
+        wp_load. wp_load. wp_apply (wp_slice_len). wp_if_destruct.
+        - wp_pures. wp_load. wp_pures. wp_load. wp_pures.
+          iPoseProof (big_sepL2_length with "[$H3_UnsatisfiedRequests]") as "%YES1".
+          iPoseProof (own_slice_small_sz with "[$H1_UnsatisfiedRequests]") as "%YES2".
+          assert (is_Some (msgv1 !! uint.nat (W64 index))) as [e H_e].
+          { eapply lookup_lt_is_Some_2. word. }
+          assert (length nexts > 0)%nat as NE_NIL.
+          { apply f_equal with (f := length) in FOCUS. rewrite length_app in FOCUS. word. }
+          destruct nexts as [ | cur nexts].
+          { simpl in NE_NIL. word. }
+          clear NE_NIL H_continue.
+          assert (s .(Server.UnsatisfiedRequests) !! index = Some cur) as H_cur.
+          { rewrite <- take_drop with (l := s .(Server.UnsatisfiedRequests)) (i := index). rewrite lookup_app_r.
+            - rewrite claim2. replace (index - length (take index s .(Server.UnsatisfiedRequests)))%nat with 0%nat.
+              + reflexivity.
+              + symmetry. rewrite length_take. word.
+            - rewrite length_take. word.
+          }
+          wp_apply (wp_SliceGet with "[$H1_UnsatisfiedRequests]"). { iPureIntro. exact H_e. } iIntros "H1_UnsatisfiedRequests".
+          wp_load. wp_apply (wp_processClientRequest (OWN_UnsatisfiedRequests := false) with "[H1_UnsatisfiedRequests H2_UnsatisfiedRequests H3_UnsatisfiedRequests H_VectorClock H_OperationsPerformed H_MyOperations H_PendingOperations H_GossipAcknowledgements H_out_going_requests]"). { admit. } admit.
+        - admit.
+      }
+      { admit. }
+      { admit. }
     }
     wp_if_destruct.
     { admit. }
